more Marshalling cleanup

disk-betree/Benchmarks.cs
@@ -229,10 +229,10 @@ class Hashing : Benchmark {
 
 class Benchmarks {
   public void RunAllBenchmarks() {
-    //new BenchmarkRandomQueries().Run();
+    new BenchmarkRandomQueries().Run();
     new BenchmarkRandomInserts().Run();
-    //new BenchmarkSequentialQueries().Run();
-    //new BenchmarkSequentialInserts().Run();
+    new BenchmarkSequentialQueries().Run();
+    new BenchmarkSequentialInserts().Run();
     //new Hashing().Run();
 
     Native_Compile.BenchmarkingUtil.dump();
